Starting circuit encoding

src/circuits/circuit_encoding.lean
@@ -4,18 +4,84 @@ import polytime.lemmas
 open tencodable tree
 open_locale tree complexity_class
 
-variables {α β : Type} [tencodable α] [tencodable β]
+section
+variables {α : Type*} {β : α → Type*}
 
-def encode_function [fintype α] : tencodable (α → β) :=
-by haveI : decidable_eq α := decidable_eq_of_encodable α; exact 
-tencodable.of_left_injection (λ f, ((finset.univ : finset α).sort lift_le).map (λ x, (⟨x, f x⟩ : Σ _ : α, β)))
-  (λ l, if H : ∀ a, a ∈ l.keys then some (λ x, option.get (list.lookup_is_some.mpr (H x))) else none) 
-  (λ b, begin
-    have : ∀ (a : α) (f : α → β), (((finset.univ : finset α).sort lift_le).map (λ x, (⟨x, f x⟩ : Σ _ : α, β))).lookup a = some (f a),
-    { intros a f, apply list.mem_lookup, { simp [list.nodupkeys, list.keys], }, simp, },
-    rw dif_pos, swap, { simp [← list.lookup_is_some, this], },
-    rw option.some_inj, ext a, simp [this],
-  end)
+lemma multiset.nodupkeys_iff {s : multiset (sigma β)} :
+  s.nodupkeys ↔ s.keys.nodup := quotient.induction_on s $ λ l, iff.rfl
 
-#check sigma.mk
+lemma finmap.keysnodup (f : finmap β) : f.entries.keys.nodup := multiset.nodupkeys_iff.mp f.nodupkeys
 
+def finmap.of_fun [fintype α] (f : Π x, β x) :
+  finmap β :=
+{ entries := finset.univ.val.map (λ x : α, ⟨x, f x⟩),
+  nodupkeys := by simpa [multiset.nodupkeys_iff, multiset.keys] using finset.univ.nodup }
+
+lemma finmap.mem_lookup_iff [decidable_eq α] {f : finmap β} {x : α} (y : β x) :
+   f.lookup x = some y ↔ (⟨x, y⟩ : sigma β) ∈ f.entries :=
+finmap.induction_on f (λ a, alist.mem_lookup_iff) 
+
+@[simp] lemma finmap.of_fun_lookup [fintype α] [decidable_eq α] {f : Π x, β x} (x : α) :
+  (finmap.of_fun f).lookup x = some (f x) :=
+by { rw finmap.mem_lookup_iff, exact multiset.mem_map_of_mem _ (finset.mem_univ_val x), }
+
+def finmap.comap {α β γ : Type*} (m : @finmap α (λ _, β)) (f : α ↪ γ) : @finmap γ (λ _, β) :=
+{ entries := m.entries.map (λ x, ⟨f x.1, x.2⟩),
+  nodupkeys := multiset.nodupkeys_iff.mpr (by simpa [multiset.keys] using m.keysnodup.map f.2) }
+
+def finmap.disj_union {α β γ : Type*} (m₁ : @finmap α (λ _, γ)) (m₂ : @finmap β (λ _, γ)) : @finmap (α ⊕ β) (λ _, γ) :=
+{ entries := m₁.entries.map (λ x, ⟨sum.inl x.1, x.2⟩) + m₂.entries.map (λ x, ⟨sum.inr x.1, x.2⟩),
+  nodupkeys := begin
+    rw [multiset.nodupkeys_iff, multiset.keys, multiset.map_add, multiset.nodup_add],
+    refine ⟨_, _, _⟩,
+    { simpa [multiset.keys] using m₁.keysnodup.map sum.inl_injective, },
+    { simpa [multiset.keys] using m₂.keysnodup.map sum.inr_injective, },
+    { simp [multiset.disjoint], }
+  end }
+
+@[simp] lemma finmap.disj_union_lookup_left {α β γ : Type*} [decidable_eq α] [decidable_eq β] (m₁ : @finmap α (λ _, γ)) (m₂ : @finmap β (λ _, γ)) (x : α) :
+  (m₁.disj_union m₂).lookup (sum.inl x) = m₁.lookup x :=
+by { ext y, simp [finmap.mem_lookup_iff, finmap.disj_union], }
+
+@[simp] lemma finmap.disj_union_lookup_right {α β γ : Type*} [decidable_eq α] [decidable_eq β] (m₁ : @finmap α (λ _, γ)) (m₂ : @finmap β (λ _, γ)) (x : β) :
+  (m₁.disj_union m₂).lookup (sum.inr x) = m₂.lookup x :=
+by { ext y, simp [finmap.mem_lookup_iff, finmap.disj_union], }
+
+def finmap.map {γ : α → Type*} (m : finmap β) (f : ∀ x, β x → γ x) : finmap γ :=
+{ entries := m.entries.map (λ x, ⟨x.1, f x.1 x.2⟩),
+  nodupkeys := by simpa [multiset.nodupkeys_iff, multiset.keys] using m.keysnodup }
+
+end
+
+variables {α β U V W X : Type}
+
+def precircuit.to_finmap [fintype V] (cct : precircuit U V) : @finmap V (λ _, list (U ⊕ V)) :=
+finmap.of_fun cct.deps
+
+def precircuit.comp_finmap (c₁ : @finmap V (λ _, list (U ⊕ V))) (c₂ : @finmap X (λ _, list (W ⊕ X))) :
+  @finmap (W ⊕ X) (λ _, list (U ⊕ V ⊕ X)) := sorry
+
+variables  [tencodable α] [tencodable β] [tencodable U] [tencodable V]
+  [tencodable W] [tencodable X]
+
+def flatten_finmap (f : @finmap V (λ _, list (U ⊕ V))) : @finmap (tree unit) (λ _, list (tree unit ⊕ tree unit)) :=
+(f.map $ λ _ l, l.map $ sum.map encode encode).comap ⟨encode, encode_injective⟩
+
+-- TODO: maybe try
+-- pcct.to_finmap : precircuit U V → finmap V (list (U ⊕ V))
+-- flatten : (finmap V (list U ⊕ V)) → finmap (tree unit) (list (tree unit) ⊕ (tree unit))
+/-
+
+polytime_dep₂ ((U : Type) → (V : Type) → M U V → N U V) → Prop where M and N are functorial in U and V
+
+
+comp_finmap : finmap V (list U ⊕ V) → finmap X (list X ⊕ W) → (f : W → U ⊕ V) → finmap (V ⊕ X) (list (U ⊕ V ⊕ X))
+
+WTS: mem (λ n, flatten (pcct₁ n).to_finmap) → mem (λ n, flatten (pcct₂ n).to_finmap) →
+  (λ n, flatten ((pcct₁ n).comp (pcct₂ n)).to_finmap)
+
+--> λ n, flatten (comp_finmap (pcct₁ n).to_finmap (pcct₂ n).to_finmap)
+
+WTS: polytime.mem $ λ (c₁ : precircuit U V) (c₂ : precircuit U V), 
+
+-/
